thys/Superposition_Calculus/Superposition.thy
@@ -82,7 +82,7 @@ inductive eq_resolution :: "('f, 'v, 'ty) typed_clause \<Rightarrow> ('f, 'v, 't
   eq_resolutionI: 
    "D = add_mset l D' \<Longrightarrow>
     l = t !\<approx> t' \<Longrightarrow>
-    welltyped_imgu \<V> t t' \<mu> \<Longrightarrow>
+    welltyped_imgu_on (clause.vars D) \<V> t t' \<mu> \<Longrightarrow>
     select D = {#} \<and> is_maximal (l \<cdot>l \<mu>) (D \<cdot> \<mu>) \<or> is_maximal (l \<cdot>l \<mu>) (select D \<cdot> \<mu>) \<Longrightarrow>
     C = D' \<cdot> \<mu> \<Longrightarrow>
     eq_resolution (D, \<V>) (C, \<V>)"
@@ -95,12 +95,11 @@ inductive eq_factoring :: "('f, 'v, 'ty) typed_clause \<Rightarrow> ('f, 'v, 'ty
     select D = {#} \<Longrightarrow> 
     is_maximal (l\<^sub>1 \<cdot>l \<mu>) (D \<cdot> \<mu>) \<Longrightarrow>
     \<not> (t\<^sub>1 \<cdot>t \<mu> \<preceq>\<^sub>t t\<^sub>1' \<cdot>t \<mu>) \<Longrightarrow>
-    welltyped_imgu \<V> t\<^sub>1 t\<^sub>2 \<mu> \<Longrightarrow>
+    welltyped_imgu_on (clause.vars D) \<V> t\<^sub>1 t\<^sub>2 \<mu> \<Longrightarrow>
     C = add_mset (t\<^sub>1 \<approx> t\<^sub>2') (add_mset (t\<^sub>1' !\<approx> t\<^sub>2') D') \<cdot> \<mu> \<Longrightarrow>
     eq_factoring (D, \<V>) (C, \<V>)"
 
 (* TODO: Get things like is_renaming out of the name scope *)
-(* TODO: \<P> \<in> {Pos, Neg} *)
 (* TODO: \<forall>x \<in> clause.vars (D \<cdot> \<rho>\<^sub>2). \<V>\<^sub>2 (inv \<rho>\<^sub>2 (Var x)) = \<V>\<^sub>3 x *)
 inductive superposition ::
   "('f, 'v, 'ty) typed_clause \<Rightarrow> ('f, 'v, 'ty) typed_clause \<Rightarrow> ('f, 'v, 'ty) typed_clause \<Rightarrow> bool"
@@ -115,7 +114,7 @@ where
     l\<^sub>1 = \<P> (Upair c\<^sub>1\<langle>t\<^sub>1\<rangle> t\<^sub>1') \<Longrightarrow>
     l\<^sub>2 = t\<^sub>2 \<approx> t\<^sub>2' \<Longrightarrow>
     \<not> is_Var t\<^sub>1 \<Longrightarrow>
-    welltyped_imgu \<V>\<^sub>3 (t\<^sub>1 \<cdot>t \<rho>\<^sub>1) (t\<^sub>2 \<cdot>t \<rho>\<^sub>2) \<mu> \<Longrightarrow>
+    welltyped_imgu_on (clause.vars (E \<cdot> \<rho>\<^sub>1) \<union> clause.vars (D \<cdot> \<rho>\<^sub>2)) \<V>\<^sub>3 (t\<^sub>1 \<cdot>t \<rho>\<^sub>1) (t\<^sub>2 \<cdot>t \<rho>\<^sub>2) \<mu> \<Longrightarrow>
     \<forall>x \<in> clause.vars (E \<cdot> \<rho>\<^sub>1). \<V>\<^sub>1 (inv \<rho>\<^sub>1 (Var x)) = \<V>\<^sub>3 x \<Longrightarrow>
     \<forall>x \<in> clause.vars (D \<cdot> \<rho>\<^sub>2). \<V>\<^sub>2 (inv \<rho>\<^sub>2 (Var x)) = \<V>\<^sub>3 x \<Longrightarrow>
     is_welltyped_on (clause.vars E) \<V>\<^sub>1 \<rho>\<^sub>1 \<Longrightarrow>
@@ -166,7 +165,7 @@ where
     l\<^sub>1 = c\<^sub>1\<langle>t\<^sub>1\<rangle> \<approx> t\<^sub>1' \<Longrightarrow>
     l\<^sub>2 = t\<^sub>2 \<approx> t\<^sub>2' \<Longrightarrow>
     \<not> is_Var t\<^sub>1 \<Longrightarrow>
-    welltyped_imgu \<V>\<^sub>3 (t\<^sub>1 \<cdot>t \<rho>\<^sub>1) (t\<^sub>2 \<cdot>t \<rho>\<^sub>2) \<mu> \<Longrightarrow>
+    welltyped_imgu_on (clause.vars (E \<cdot> \<rho>\<^sub>1) \<union> clause.vars (D \<cdot> \<rho>\<^sub>2)) \<V>\<^sub>3 (t\<^sub>1 \<cdot>t \<rho>\<^sub>1) (t\<^sub>2 \<cdot>t \<rho>\<^sub>2) \<mu> \<Longrightarrow>
     \<forall>x \<in> clause.vars (E \<cdot> \<rho>\<^sub>1). \<V>\<^sub>1 (inv \<rho>\<^sub>1 (Var x)) = \<V>\<^sub>3 x \<Longrightarrow>
     \<forall>x \<in> clause.vars (D \<cdot> \<rho>\<^sub>2). \<V>\<^sub>2 (inv \<rho>\<^sub>2 (Var x)) = \<V>\<^sub>3 x \<Longrightarrow>
     is_welltyped_on (clause.vars E) \<V>\<^sub>1 \<rho>\<^sub>1 \<Longrightarrow>
@@ -207,7 +206,7 @@ where
     l\<^sub>1 = c\<^sub>1\<langle>t\<^sub>1\<rangle> !\<approx> t\<^sub>1' \<Longrightarrow>
     l\<^sub>2 = t\<^sub>2 \<approx> t\<^sub>2' \<Longrightarrow>
     \<not> is_Var t\<^sub>1 \<Longrightarrow>
-    welltyped_imgu \<V>\<^sub>3 (t\<^sub>1 \<cdot>t \<rho>\<^sub>1) (t\<^sub>2 \<cdot>t \<rho>\<^sub>2) \<mu> \<Longrightarrow>
+    welltyped_imgu_on (clause.vars (E \<cdot> \<rho>\<^sub>1) \<union> clause.vars (D \<cdot> \<rho>\<^sub>2)) \<V>\<^sub>3 (t\<^sub>1 \<cdot>t \<rho>\<^sub>1) (t\<^sub>2 \<cdot>t \<rho>\<^sub>2) \<mu> \<Longrightarrow>
     \<forall>x \<in> clause.vars (E \<cdot> \<rho>\<^sub>1). \<V>\<^sub>1 (inv \<rho>\<^sub>1 (Var x)) = \<V>\<^sub>3 x \<Longrightarrow>
     \<forall>x \<in> clause.vars (D \<cdot> \<rho>\<^sub>2). \<V>\<^sub>2 (inv \<rho>\<^sub>2 (Var x)) = \<V>\<^sub>3 x \<Longrightarrow>
     is_welltyped_on (clause.vars E) \<V>\<^sub>1 \<rho>\<^sub>1 \<Longrightarrow>
