thys/Superposition_Calculus/Superposition_Soundness.thy
@@ -44,7 +44,7 @@ proof (cases D C rule: eq_resolution.cases)
     let ?t\<^sub>G = "term.to_ground (t \<cdot>t \<mu> \<cdot>t \<gamma>')"
     let ?t\<^sub>G' = "term.to_ground (t' \<cdot>t \<mu> \<cdot>t \<gamma>')"
 
-    have \<mu>_is_welltyped: "is_welltyped \<V> \<mu>"
+    have \<mu>_is_welltyped: "is_welltyped_on (clause.vars D) \<V> \<mu>"
       using eq_resolutionI
       by meson
 
@@ -154,7 +154,7 @@ proof (cases D C rule: eq_factoring.cases)
     let ?t\<^sub>G\<^sub>2' = "term.to_ground (t\<^sub>2' \<cdot>t \<mu> \<cdot>t \<gamma>')"
     let ?C\<^sub>G = "clause.to_ground (C \<cdot> \<gamma>')"
 
-    have \<mu>_is_welltyped: "is_welltyped \<V> \<mu>"
+    have \<mu>_is_welltyped: "is_welltyped_on (clause.vars D) \<V> \<mu>"
       using eq_factoringI(9)
       by blast
 
@@ -306,7 +306,7 @@ proof (cases D E C rule: superposition.cases)
       "term_subst.is_ground_subst (\<mu> \<odot> \<gamma>')"
       using term.is_ground_subst_comp_right[OF \<gamma>'_is_ground_subst].
 
-    have \<mu>_is_welltyped: "is_welltyped \<V>\<^sub>3 \<mu>"
+    have \<mu>_is_welltyped: "is_welltyped_on (clause.vars (E \<cdot> \<rho>\<^sub>1) \<union> clause.vars (D \<cdot> \<rho>\<^sub>2)) \<V>\<^sub>3 \<mu>"
       using superpositionI(13)
       by blast
 
@@ -320,12 +320,11 @@ proof (cases D E C rule: superposition.cases)
           superposition[unfolded superpositionI(1-3)] 
           C_is_welltyped].
 
-    have is_welltyped_\<mu>_\<gamma>: "is_welltyped \<V>\<^sub>3 (\<mu> \<odot> \<gamma>')"
+    have is_welltyped_\<mu>_\<gamma>: "is_welltyped_on (clause.vars (E \<cdot> \<rho>\<^sub>1) \<union> clause.vars (D \<cdot> \<rho>\<^sub>2)) \<V>\<^sub>3 (\<mu> \<odot> \<gamma>')"
       using \<gamma>'_is_welltyped \<mu>_is_welltyped
-      by (simp add: is_welltyped_subst_compose)
+      by (simp add: is_welltyped_on_subst_compose)
 
-    note is_welltyped_\<rho>_\<mu>_\<gamma> = welltyped.renaming_ground_subst[OF 
-        _ is_welltyped_\<mu>_\<gamma> _ \<mu>_\<gamma>'_is_ground_subst]
+    note is_welltyped_\<rho>_\<mu>_\<gamma> = welltyped.renaming_ground_subst[OF _ _ _ \<mu>_\<gamma>'_is_ground_subst]
 
     have "?E\<^sub>G \<in> clause_groundings (E, \<V>\<^sub>1)"
     proof(
@@ -335,15 +334,18 @@ proof (cases D E C rule: superposition.cases)
       show "clause.to_ground (E \<cdot> \<rho>\<^sub>1 \<cdot> \<mu> \<cdot> \<gamma>') = clause.to_ground (E \<cdot> \<rho>\<^sub>1 \<odot> \<mu> \<odot> \<gamma>')"
         by simp
     next
+
       show "clause.is_ground (E \<cdot> \<rho>\<^sub>1 \<odot> \<mu> \<odot> \<gamma>')"  
         using \<gamma>'_is_ground_subst clause.is_ground_subst_is_ground
         by auto
     next
+
       show "is_welltyped_on (clause.vars E) \<V>\<^sub>1 (\<rho>\<^sub>1 \<odot> \<mu> \<odot> \<gamma>')"
         using
-          is_welltyped_\<rho>_\<mu>_\<gamma>[OF 
-            superpositionI(4, 16) superpositionI(14)[unfolded clause.vars_subst]]
-        by (simp add: subst_compose_assoc)
+          is_welltyped_\<mu>_\<gamma>
+          is_welltyped_\<rho>_\<mu>_\<gamma>[OF
+            superpositionI(4) _  superpositionI(16, 14)[unfolded clause.vars_subst]]
+        by (simp add: subst_compose_assoc clause.vars_subst)
     qed
 
     then have entails_E\<^sub>G: "?I \<TTurnstile> ?E\<^sub>G"
@@ -362,11 +364,13 @@ proof (cases D E C rule: superposition.cases)
         using \<gamma>'_is_ground_subst clause.is_ground_subst_is_ground
         by auto
     next
+
       show "is_welltyped_on (clause.vars D) \<V>\<^sub>2 (\<rho>\<^sub>2 \<odot> \<mu> \<odot> \<gamma>')"
-        using
-          is_welltyped_\<rho>_\<mu>_\<gamma>[OF 
-            superpositionI(5, 17) superpositionI(15)[unfolded clause.vars_subst]]
-        by (simp add: subst_compose_assoc)
+        using 
+          is_welltyped_\<mu>_\<gamma>
+          is_welltyped_\<rho>_\<mu>_\<gamma>[OF
+            superpositionI(5) _ superpositionI(17, 15)[unfolded clause.vars_subst]]
+        by (simp add: subst_compose_assoc clause.vars_subst)
     qed
 
     then have entails_D\<^sub>G: "?I \<TTurnstile> ?D\<^sub>G"
